examples/dynamic_isolation/Framework.v
@@ -1,0 +1,60 @@
+Require Import dynamic_isolation.Tactics.
+Require Import Coq.Lists.List.
+Import ListNotations.
+
+Section StepFramework.
+  Section Parameterised.
+    Context {state_t event_t: Type}.
+    Context (initial_state: state_t).
+    Context (step_fn: state_t -> state_t * event_t).
+
+    Fixpoint step_n (n: nat) : state_t * list event_t :=
+      match n with
+      | 0 => (initial_state, [])
+      | S n' =>
+          let (st, evs) := step_n n' in
+          let (st', ev) := step_fn st in
+          (st', evs ++ [ev])
+      end.
+
+  End Parameterised.
+
+  Section Projection.
+    Context {state_t event_t: Type}.
+    Context {state_t' : Type}.
+    Context (initial_state: state_t).
+    Context (initial_state': state_t').
+    Context (step_fn: state_t -> state_t * event_t).
+    Context (step_fn': state_t' -> state_t' * event_t).
+    Context (proj_st: state_t -> state_t').
+    (* Context (pf_proj_initial: proj_st initial_state = initial_state'). *)
+
+    Definition is_proj (st: state_t) (st': state_t') : Prop :=
+      proj_st st = st'.
+
+    Definition natural_step_fn :=
+      forall st st',
+      is_proj st st' ->
+      is_proj (fst (step_fn st)) (fst (step_fn' st')) /\ (snd (step_fn st) = snd (step_fn' st')).
+
+    Context (pf_proj_initial: is_proj initial_state initial_state').
+    Context (pf_natural_step: natural_step_fn).
+
+    Lemma proj_step_fn_eq: forall (n: nat) (st: state_t) (st': state_t') (evs evs': list event_t),
+      step_n initial_state step_fn n = (st, evs) ->
+      step_n initial_state' step_fn' n = (st', evs') ->
+      st' = proj_st st /\ evs = evs'.
+    Proof.
+      induction n; intros; simplify_all.
+      destruct_all_matches; simplify_all.
+      specialize IHn with (1 := eq_refl) (2 := eq_refl); propositional; subst.
+      consider natural_step_fn.
+      specialize pf_natural_step with (st := s1) (st' := proj_st s1).
+      rewrite Heqp2 in *. rewrite Heqp0 in *. simpl in *.
+      consider is_proj.
+      destruct pf_natural_step; subst; auto.
+    Qed.
+
+  End Projection.
+
+End StepFramework.
